\begin{small}
  \begin{mathpar}
\infer{
\Gamma, x : T \vdash x : T
}{}
\qquad
\infer{
\Gamma \vdash k : \bbbc
}{
k \in \mathbb{Z}
}
\qquad
\infer{
\Gamma \vdash E_1 + E_2 : \bbbc
}{
\Gamma \vdash E_1 : \bbbc
&
\Gamma \vdash E_2 : \bbbc
}
\qquad
\infer{
\Gamma \vdash () : 1
}{}

\\

\infer{
\Gamma \vdash E_1 \; E_2 : T_2
}{
\Gamma \vdash E_1 : T_1 \to T_2
&
\Gamma \vdash E_2 : T_1
}
\qquad
\infer{
\Gamma \vdash \lambda x.E : T_1 \to T_2
}{
\Gamma, x : T_1 \vdash E : T_2
}
\qquad
\infer{
\Gamma \vdash (E_1,E_2) : T_1 \times T_2
}{
\Gamma \vdash E_1 : T_1
&
\Gamma \vdash E_2 : T_2
}
\qquad
\infer{
\Gamma \vdash \pi_i E : T_i
}{
\Gamma \vdash E : T_1 \times T_2
}

\\

\infer{
\Gamma \vdash \inl E : T_1 + T_2
}{
\Gamma \vdash E : T_1
}
\qquad
\infer{
\Gamma \vdash \inr E : T_1 + T_2
}{
\Gamma \vdash E : T_2
}
\qquad
\infer{
\Gamma \vdash \ccase E x {E_1} y {E_2} : T
}{
\Gamma \vdash E : T_1 + T_2
&
\Gamma, x : T_1 \vdash E_1 : T
&
\Gamma, y : T_2 \vdash E_2 : T
}

\\

\infer{
\Gamma \vdash 0 : \N
}{}
\qquad
\infer{
\Gamma \vdash S(E) : \N
}{
\Gamma \vdash E : \N
}
\qquad
\infer{
\Gamma \vdash \nrec {E} {E_1} {E_2} : T
}{
\Gamma \vdash E : \N
&
\Gamma \vdash E_1 : 1 \to T
&
\Gamma \vdash E_2 : \N \times T \to T
}

\\

\infer{
\Gamma \vdash \elist : \listty T
}{}
\qquad
\infer{
\Gamma \vdash \cons {E_1} {E_2} : \listty T
}{
\Gamma \vdash E_1 : T
&
\Gamma \vdash E_2 : \listty T
}
\qquad
\infer{
\Gamma \vdash \lrec E {E_1} {E_2} : T
}{
  \begin{array}{l}
    \Gamma \vdash E : \listty {T_1}\\
\Gamma \vdash E_1 : 1 \to T\\
\Gamma \vdash E_2 : T_1\times(\listty {T_1} \times T) \to T
  \end{array}
}
\end{mathpar}
\end{small}
