% \begin{small}
% \[
% \begin{array}{l}
% \norm{A} = \bbbc \times \angles{A} \\
% \angles{!^k_\ell A} = \angles{A} \\
% \angles{1} = 1 \\
% \angles{A \otimes B} = \angles{A} \times \angles{B} \\
% \angles{A \oplus B} = \angles{A} + \angles{B} \\
% \angles{A \loli B} = \angles{A} \to \norm{B} \\
% \angles{A \amp B} = \norm{A} \times \norm{B} \\
% \angles{\N} = \N \\
% \angles{\listty A} = \listty {\angles A} \\
% \\
% \norm{x} = (0,x)\\
% \norm{()} = (0,())\\
% \norm{\tick M} = 1 +_c \norm{M}\\
% \norm{(M,N)} = (\norm{M}_c + \norm{N}_c,(\norm{M}_p,\norm{N}_p))\\
% \norm{\asplit {k'} M x y N} = k'\norm{M}_c +_c \norm{N}[\pi_1\norm{M}_p/x,\pi_2\norm{M}_p/y]\\
% \norm{\lambda x.M} = (0,\lambda x.\norm{M})\\
% \norm{M \; N} = (\norm{M}_c + \norm{N}_c) +_c \norm{M}_p \; \norm{N}_p\\
% \norm{\inl M} = (\norm{M}_c,\inl {\norm{M}_p})\\
% \norm{\inr M} = (\norm{M}_c,\inr {\norm{M}_p})\\
% \norm{\acase {k'} M x {N_1} y {N_2}} = k'\norm{M}_c + \ccase {\norm{M}_p} x {\norm{N_1}} y {\norm{N_2}}\\
% \norm{0} = (0,0)\\
% \norm{S(M)} = (\norm{M}_c,S(\norm{M}_p))\\
% \norm{\elist} = (0,\elist)\\
% \norm{\cons M N} = (\norm{M}_c + \norm{N}_c,\cons {\norm{M}_p} {\norm{N}_p})\\
% \norm{\tsfer {k'} k \ell x M N} = k'\norm{M}_c +_c \norm{N}[\norm{M}_p/x]\\
% \norm{\save k \ell M} = (k\norm{M}_c,\norm{M}_p)\\
% \norm{\wait \ell M} = \ell +_c \norm{M}\\
% \norm{\disc \ell M} = (-\ell) +_c \norm{M}\\
% \norm{\amppair M N} = (0,(\norm{M},\norm{N}))\\
% \norm{\pi_i M} = \norm{M}_c +_c \pi_i\left(\norm{M}_p\right)\\
% \norm{\nrec M {N_1} {N_2}} = (\norm{M}_c + \norm{N_1}_c + \norm{N_2}_c) +_c \nrec {\norm{M}_p} {\norm{N_1}_p} {\lambda x. \norm{N_2}_p(\pi_1 x,\lambda z.\pi_2 x)}\\
% \norm{\lrec M {N_1} {N_2}}=(\norm{M}_c+\norm{N_1}_c+\norm{N_2}_c)+_c\lrec {\norm{M}_p} {\norm{N_1}_p} {\lambda x. \norm{N_2}_p (\pi_1 x,((0,\pi_1 \pi_2 x),\pi_2\pi_2 x)) }\\
% \end{array}
% \]
% \end{small}

\begin{small}
\[
\begin{array}{c}
\norm{A} = \bbbc \times \angles{A} \\
\angles{1} = 1 \qquad
\angles{A \otimes B} = \angles{A} \times \angles{B}\qquad
\angles{A \oplus B} = \angles{A} + \angles{B}\qquad
\angles{A \loli B} = \angles{A} \to \norm{B} \\
\angles{!^k_\ell A} = \angles{A} \qquad
\angles{A \amp B} = \norm{A} \times \norm{B} \\
\angles{\N} = \N\qquad
\angles{\listty A} = \listty {\angles A} \\
\end{array}
\]

\[
\begin{array}{c}
\norm{x} = (0,x) \\
\norm{()} = (0,()) \qquad
\norm{(M,N)} = (\norm{M}_c + \norm{N}_c,(\norm{M}_p,\norm{N}_p)) \qquad
\norm{\pi_i M} = \norm{M}_c +_c \pi_i\left(\norm{M}_p\right)\\ \\
\norm{\inl M} = (\norm{M}_c,\inl {\norm{M}_p}) \qquad
\norm{\inr M} = (\norm{M}_c,\inr {\norm{M}_p})\\
\norm{\acase {k'} M x {N_1} y {N_2}} = k'\norm{M}_c + \ccase {\norm{M}_p} x {\norm{N_1}} y {\norm{N_2}}\\ \\
\norm{\lambda x.M} = (0,\lambda x.\norm{M}) \qquad
\norm{M \; N} = (\norm{M}_c + \norm{N}_c) +_c \norm{M}_p \; \norm{N}_p\\ \\
\norm{\amppair M N} = (0,(\norm{M},\norm{N}))\\
\norm{\asplit {k'} M x y N} = k'\norm{M}_c +_c \norm{N}[\pi_1\norm{M}_p/x,\pi_2\norm{M}_p/y]\\ \\
\norm{0} = (0,0) \qquad
\norm{S(M)} = (\norm{M}_c,S(\norm{M}_p)) \\ \\
\norm{\elist} = (0,\elist) \qquad
\norm{\cons M N} = (\norm{M}_c + \norm{N}_c,\cons {\norm{M}_p} {\norm{N}_p}) \\ \\
\norm{\tick M} = 1 +_c \norm{M}\\
\norm{\tsfer {k'} k \ell x M N} = k'\norm{M}_c +_c \norm{N}[\norm{M}_p/x] \qquad
\norm{\save k \ell M} = (k\norm{M}_c,\norm{M}_p)\\
\norm{\wait \ell M} = \ell +_c \norm{M} \qquad
\norm{\disc \ell M} = (-\ell) +_c \norm{M}\\ \\
\norm{\nrec M {N_1} {N_2}} = (\norm{M}_c + \norm{N_1}_c + \norm{N_2}_c) +_c \nrec {\norm{M}_p} {\norm{N_1}_p} {\lambda x. \norm{N_2}_p(\pi_1 x,\lambda z.\pi_2 x)}\\
\hspace{-10em}\norm{\lrec M {N_1} {N_2}}=(\norm{M}_c+\norm{N_1}_c+\norm{N_2}_c)+_c\\
\hspace{12em}\lrec {\norm{M}_p} {\norm{N_1}_p} {\lambda x. \norm{N_2}_p (\pi_1 x,((0,\pi_1 \pi_2 x),\pi_2\pi_2 x)) }\\
\end{array}
\]
\end{small}
