\jtheorem{Proof of \autoref{thm:raw-constr-idx-subst}}{
  \jgivengoal{
    \caseFact{1} $\Theta, i : S ; \Delta \vdash \Phi \, \texttt{wf}$
    
    \caseFact{2} $\Theta ; \Delta \vdash I : S$
  }{
     $\Theta ; \Delta[I/i] \pvdash \Phi[I/i] \, \texttt{wf}$
  }
  
  \jcase{1}{C-Top}{Immediate.}
  \jcase{2}{C-Bot}{Immediate.}
  \jcase{3}{C-Conj}{
    \jgivengoal{
      \caseFact{1} $\Theta, i : S ; \Delta \vdash \Phi_1 \wedge \Phi_2 \, \texttt{wf}$
      
      \caseFact{3} $\Theta, i : S ; \Delta \vdash \Phi_1 \, \texttt{wf}$
      
      \caseFact{4} $\Theta, i : S ; \Delta \vdash \Phi_2 \, \texttt{wf}$
    }{$\Theta ; \Delta \pvdash (\Phi_1 \wedge \Phi_2)[I/i] \, \texttt{wf}$}
      \caseText{By IH on (3) and (4)}
      
      \caseFact{5} $\Theta ; \Delta[I/i] \vdash \Phi_1[I/i] \, \texttt{wf}$
      
      \caseFact{6} $\Theta ; \Delta[I/i] \vdash \Phi_2[I/i] \, \texttt{wf}$
      
      \caseText{The result follows by C-Conj on (5) and (6)}
  }
  \jcase{4}{C-Disj}{
    \jgivengoal{
      \caseFact{1} $\Theta, i : S ; \Delta \vdash \Phi_1 \vee \Phi_2 \, \texttt{wf}$
      
      \caseFact{3} $\Theta, i : S ; \Delta \vdash \Phi_1 \, \texttt{wf}$
      
      \caseFact{4} $\Theta, i : S ; \Delta \vdash \Phi_2 \, \texttt{wf}$
    }{$\Theta ; \Delta \pvdash (\Phi_1 \vee \Phi_2)[I/i] \, \texttt{wf}$}
      \caseText{By IH on (3) and (4)}
      
      \caseFact{5} $\Theta ; \Delta[I/i] \vdash \Phi_1[I/i] \, \texttt{wf}$
      
      \caseFact{6} $\Theta ; \Delta[I/i] \vdash \Phi_2[I/i] \, \texttt{wf}$
      
      \caseText{The result follows by C-Disj on (5) and (6)}
  }
  \jcase{5}{C-Impl}{
    \jgivengoal{
      \caseFact{1} $\Theta, i : S ; \Delta \vdash \Phi_1 \to \Phi_2 \, \texttt{wf}$
      
      \caseFact{3} $\Theta, i : S ; \Delta \vdash \Phi_1 \, \texttt{wf}$
      
      \caseFact{4} $\Theta, i : S ; \Delta, \Phi_1 \vdash \Phi_2 \, \texttt{wf}$
    }{$\Theta ; \Delta[I/i] \vdash (\Phi_1 \vee \Phi_2)[I/i] \, \texttt{wf}$}
      \caseText{By IH on (3) and (4)}
      
      \caseFact{5} $\Theta ; \Delta[I/i] \vdash \Phi_1[I/i] \, \texttt{wf}$
      
      \caseFact{6} $\Theta ; \Delta[I/i], \Phi_1[I/i] \vdash \Phi_2[I/i] \, \texttt{wf}$
      
      \caseText{By C-Impl on (5) and (6)}
      
      \caseFact{7} $\Theta ; \Delta[I/i] \vdash \Phi_1[I/i] \to \Phi_2[I/i] \, \texttt{wf}$
      
      \caseText{The result follows by C-Disj on (5) and (6)}
  }
  
  \jcase{6}{C-Forall}{
   \jgivengoal{
     \caseFact{1} $\Theta, i : S ; \Delta \vdash \forall j : S'. \Phi \, \texttt{wf}$
     
     \caseFact{3} $\Theta, i : S, j : S' ; \Delta \vdash \Phi \, \texttt{wf}$
   }{$\Theta ; \Delta[I/i] \vdash (\forall j : S'.\Phi)[I/i]$}
   
   \caseText{By IH on (3)}
   
   \caseFact{4} $\Theta, j : S' ; \Delta[I/i] \vdash \Phi[I/i] \, \texttt{wf}$
   
   \caseText{By C-Forall on (4)}
   
   \caseFact{5} $\Theta ; \Delta[I/i] \vdash \forall j : S'. \Phi[I/i] \, \texttt{wf}$
   
   \caseText{The goal follows by (5)}
  }
  
  \jcase{6}{C-Exists}{
   \jgivengoal{
     \caseFact{1} $\Theta, i : S ; \Delta \vdash \exists j : S'. \Phi \, \texttt{wf}$
     
     \caseFact{3} $\Theta, i : S, j : S' ; \Delta \vdash \Phi \, \texttt{wf}$
   }{$\Theta ; \Delta[I/i] \vdash (\exists j : S'.\Phi)[I/i]$}
   
   \caseText{By IH on (3)}
   
   \caseFact{4} $\Theta, j : S' ; \Delta[I/i] \vdash \Phi[I/i] \, \texttt{wf}$
   
   \caseText{By C-Exists on (4)}
   
   \caseFact{5} $\Theta ; \Delta[I/i] \vdash \exists j : S'. \Phi[I/i] \, \texttt{wf}$
   
   \caseText{The goal follows by (5)}
  }
  
  \jcase{7}{C-Eq}{\caseText{Immediate by \autoref{thm:raw-idx-idx-subst}.}}
  
  \jcase{8}{C-Leq}{\caseText{Immediate by \autoref{thm:raw-idx-idx-subst}.}}
  
  \jcase{9}{C-Lt}{\caseText{Immediate by \autoref{thm:raw-idx-idx-subst}.}}
}