\begin{proof}
By induction on $\Theta;\Delta \vdash I : S \gens \Phi$.
\begin{enumerate}
  \item[AI-Var] Immediate.
  \item[AI-Plus] Suppose $\Theta ;\Delta \vdash I + J : bS \gens \Phi_1 \wedge \Phi_2$ and $\Theta ; \Delta \vdash I : bS \gens \Phi_1$, $\Theta ; \Delta \vdash J : bS \gens \Phi_2$. Since $\Theta ; \Delta \vDash \Phi_1 \wedge \Phi_2$, $\Theta ; \Delta \vDash \Phi_i$ for $i=1,2$. Then by IH, $\Theta ; \Delta \vdash I : bS$ and $\Theta ; \Delta \vdash J : bS$, and so by I-Plus, $\Theta ; \Delta \vdash I + J : bS$, as required.
  \item[AI-Minus] Suppose $\Theta ;\Delta \vdash I - J : bS \gens \Phi_1 \wedge \Phi_2 \wedge (I \geq J)$ and $\Theta ; \Delta \vdash I : bS \gens \Phi_1$, $\Theta ; \Delta \vdash J : bS \gens \Phi_2$. Since $\Theta ; \Delta \vDash \Phi_i$ for $i=1,2$, we have by IH that $\Theta ; \Delta \vdash I : bS$ and $\Theta ; \Delta \vdash J : bS$. Further, $\Theta ; \Delta \vDash I \geq J$, and so by I-Minus, $\Theta ;\Delta \vdash I - J : bS$, as required.
  \item[AI-Times-*] Immediate by IH.
  \item[AI-Shift] Immediate by IH.
  \item[AI-Lam] Suppose $\Theta ; \Delta \vdash \lambda i : bS. I : bS \to S \gens \Phi$ by way of $\Theta , i : bS ; \Delta \vdash i : S \gens \Phi$, and $\Theta ; \Delta \vDash \Phi$. By IH, $\Theta, i : bS ; \Delta \vdash I : S$, and so by I-Lam, $\Theta ; \Delta \vdash \lambda i : bS. I : bS \to S$.
  \item[AI-App] Suppose $\Theta ;\Delta \vdash I\; J : S \gens \Phi_1 \wedge \Phi_2$ by way of $\Theta ; \Delta \vdash I : bS \to S \gens \Phi_1$, and $\Theta ; \Delta \vDash J ; bS \gens \Phi_i$ with $i=1,2$. By IH, $\Theta ; \Delta \vdash I : bS \to S$, and $\Theta ; \Delta \vdash J : bS$. Then, by I-App, $\Theta ; \Delta \vdash I \; J : S$, as required.
  \item[AI-Sum] Suppose $\Theta;\Delta \vdash \sum_{i=I_0}^{I_1} J : bS \gens \Phi_1 \wedge \Phi_2 \wedge \forall i : \N.(I_0 \leq i \leq I_1 \to \Phi_3)$ by way of $\Theta;\Delta \vdash I_0 : \mathbb{N} \gens \Phi_1$, $\Theta;\Delta \vdash I_1 : \mathbb{N} \gens \Phi_2$, and $\Theta,i : \N;\Delta, I_0 \leq i \leq I_1 \vdash J : bS \gens \Phi_3$, and 
  $\Theta ; \Delta \vDash \Phi_1$,
  $\Theta ; \Delta \vDash \Phi_2$, and 
  $\Theta ; \Delta \vDash \forall i : \N.(I_0 \leq i \leq I_1 \to \Phi_3)$. By using the IH twice, $\Theta ; \Delta \vdash I_i : \N$ for $i=1,2$. We note that   $\Theta ; \Delta \vDash \forall i : \N.(I_0 \leq i \leq I_1 \to \Phi_3)$ is equivalent to $\Theta, i : \N ; \Delta, I_0 \leq i \leq I_1 \vDash \Phi_3$, and so by IH, $\Theta,i : \N;\Delta, I_0 \leq i \leq I_1 \vdash J : bS$. Applying I-Sum, we have $\Theta;\Delta \vdash \sum_{i=I_0}^{I_1} J : bS$, as required.
  \item[AI-*-Lit] Immediate.
\end{enumerate}
\end{proof}