\begin{proof}
 We proceed by induction on $\Psi ; \Theta ; \Delta \vdash \tau_1 \subtynf \tau_2 : K \gens \Phi$.

\begin{itemize}
  \item[AS-Unit] Immediate.
  \item[AS-Var] Immediate.
  \item[AS-Arr] Suppose $\Psi ; \Theta ; \Delta \vdash \tau_1 \loli \tau_2 \subtynf \tau_1' \loli \tau_2' : \star \gens \Phi_1 \wedge \Phi_2$ by way of $\Psi ; \Theta ; \Delta \vdash \tau_1' \subtynf \tau_1 : \star \gens \Phi_1$ and $\Psi ; \Theta ; \Delta \vdash \tau_2 \subtynf \tau_2' : \star \gens \Phi_2$, with $\Theta ; \Delta \vDash \Phi_1 \wedge \Phi_2$. By IH, $\Psi ; \Theta ; \Delta \vdash \tau_1' \subty \tau_1 : \star$ and $\Psi ; \Theta ; \Delta \vdash \tau_2 \subty \tau_2' : \star$. By S-Arr, $\Psi ; \Theta ; \Delta \vdash \tau_1 \loli \tau_2 \subty \tau_1' \loli \tau_2' : \star$.
  \item[AS-Tensor] Suppose $\Psi ; \Theta ; \Delta \vdash \tau_1 \otimes \tau_2 \subtynf \tau_1' \otimes \tau_2' : \star \gens \Phi_1 \wedge \Phi_2$ by way of $\Psi ; \Theta ; \Delta \vdash \tau_1 \subtynf \tau_1' : \star  \gens \Phi_1$ and $\Psi ; \Theta ; \Delta \vdash \tau_2 \subtynf \tau_2' : \star \gens \Phi_2$, with $\Theta ; \Delta \vDash \Phi_1 \wedge \Phi_2$. By IH, $\Psi ; \Theta ; \Delta \vdash \tau_1 \subty \tau_1' : \star$ and $\Psi ; \Theta ; \Delta \vdash \tau_2 \subty \tau_2' : \star$, and so by S-Tensor, $\Psi ; \Theta ; \Delta \vdash \tau_1 \otimes \tau_2 \subty \tau_1' \otimes \tau_2' : \star$ as required.
  \item[AS-With] Suppose $\Psi ; \Theta ; \Delta \vdash \tau_1 \amp \tau_2 \subtynf \tau_1' \amp \tau_2' : \star \gens \Phi_1 \wedge \Phi_2$ by way of $\Psi ; \Theta ; \Delta \vdash \tau_1 \subtynf \tau_1' : \star  \gens \Phi_1$ and $\Psi ; \Theta ; \Delta \vdash \tau_2 \subtynf \tau_2' : \star \gens \Phi_2$, with $\Theta ; \Delta \vDash \Phi_1 \wedge \Phi_2$. By IH, $\Psi ; \Theta ; \Delta \vdash \tau_1 \subty \tau_1' : \star$ and $\Psi ; \Theta ; \Delta \vdash \tau_2 \subty \tau_2' : \star$, and so by S-With, $\Psi ; \Theta ; \Delta \vdash \tau_1 \amp \tau_2 \subty \tau_1' \amp \tau_2' : \star$ as required.
  \item[AS-Sum] Suppose $\Psi ; \Theta ; \Delta \vdash \tau_1 \oplus \tau_2 \subtynf \tau_1' \oplus \tau_2' : \star \gens \Phi_1 \wedge \Phi_2$ by way of $\Psi ; \Theta ; \Delta \vdash \tau_1 \subtynf \tau_1' : \star  \gens \Phi_1$ and $\Psi ; \Theta ; \Delta \vdash \tau_2 \subtynf \tau_2' : \star \gens \Phi_2$, with $\Theta ; \Delta \vDash \Phi_1 \wedge \Phi_2$. By IH, $\Psi ; \Theta ; \Delta \vdash \tau_1 \subty \tau_1' : \star$ and $\Psi ; \Theta ; \Delta \vdash \tau_2 \subty \tau_2' : \star$, and so by S-Sum, $\Psi ; \Theta ; \Delta \vdash \tau_1 \oplus \tau_2 \subty \tau_1' \oplus \tau_2' : \star$ as required.
  \item[AS-Bang] Suppose $\Psi ; \Theta ; \Delta \vdash !\tau_1 \subtynf !\tau_2 : \star \gens \Phi$ by way of $\Psi ; \Theta ; \Delta \vdash \tau_1 \subtynf \tau_2 : \star \gens \Phi$ with $\Theta ; \Delta \vDash \Phi$. By IH, $\Psi ; \Theta ; \Delta \vdash \tau_1 \subty \tau_2 : \star$, and so by S-Bang, $\Psi ; \Theta ; \Delta \vdash !\tau_1 \subty !\tau_2 : \star$ as required.
  \item[AS-IForall] Suppose $\Psi ; \Theta ; \Delta \vdash \forall i : S. \tau_1 \subtynf \forall i : S. \tau_2 : \star \gens \forall i : S. \Phi$ by way of $\Psi ; \Theta, i : S ; \Delta \vdash \tau_1 \subtynf \tau_2 : \star \gens \Phi$ with $\Theta ; \Delta \vDash \forall i : S. \Phi$. Equivalently, $\Theta, i : S; \Delta \vDash \Phi$. So, by IH, $\Psi ; \Theta, i : S ; \Delta \vdash \tau_1 \subty \tau_2 : \star$, and so by S-IForall, $\Psi ; \Theta ; \Delta \vdash \forall i : S. \tau_1 \subty \forall i : S. \tau_2 : \star$.
  \item[AS-IExists] Suppose $\Psi ; \Theta ; \Delta \vdash \exists i : S. \tau_1 \subtynf \exists i : S. \tau_2 : \star \gens \forall i : S. \Phi$ by way of $\Psi ; \Theta, i : S ; \Delta \vdash \tau_1 \subtynf \tau_2 : \star \gens \Phi$ with $\Theta ; \Delta \vDash \forall i : S. \Phi$. Equivalently, $\Theta, i : S; \Delta \vDash \Phi$. So, by IH, $\Psi ; \Theta, i : S ; \Delta \vdash \tau_1 \subty \tau_2 : \star$, and so by S-IExists, $\Psi ; \Theta ; \Delta \vdash \exists i : S. \tau_1 \subty \exists` i : S. \tau_2 : \star$.
  \item[AS-TForall] Suppose $\Psi ; \Theta ; \Delta \vdash \forall \alpha : K. \tau_1 \subtynf \forall \alpha : K. \tau_2 : \star \gens \Phi$ by way of $\Psi, \alpha : K ; \Theta ; \Delta \vdash \tau_1 \subtynf \tau_2 : \star \gens \Phi$, with $\Theta ; \Delta \vDash \Phi$. By IH, $\Psi, \alpha : K ; \Theta ; \Delta \vdash \tau_1 \subty \tau_2 : \star$. By S-TForall, $\Psi ; \Theta ; \Delta \vdash \forall \alpha : K. \tau_1 \subty \forall \alpha : K. \tau_2 : \star$, as required.
  \item[AS-List] Suppose $\Psi ; \Theta ; \Delta \vdash L^I \tau_1 \subtynf L^J \tau_2 : \star \gens I = J \wedge \Phi$ by way of $\Psi ; \Theta ; \Delta \vdash \tau_1 \subtynf \tau_2 : \star \gens \Phi$, with $\Theta ; \Delta \vDash I = J \wedge \Phi$. Equivalently, $\Theta ; \Delta \vDash I = J$ and $\Theta ; \Delta \vDash \Phi$. So, by IH, $\Psi ; \Theta ; \Delta \vdash \tau_1 \subty \tau_2 : \star$, and so because $\Theta ; \Delta \vDash I = J$, $\Psi ; \Theta ; \Delta \vdash L^I \tau_1 \subty L^J \tau_2 : \star$, as required.
  \item[AS-Impl] Suppose $\Psi ; \Theta ; \Delta \vdash \Phi_1 \implies \tau_1 \subtynf \Phi_2 \implies \tau_2 : \star \gens \Phi \wedge (\Phi_2 \to \Phi_1)$ by way of $\Psi ; \Theta ; \Delta \vdash \tau_1 \subtynf \tau_2 : \star \gens \Phi$ with $\Theta ; \Delta \vDash \Phi$ and $\Theta ; \Delta \vDash \Phi_2 \to \Phi_1$. By IH, $\Psi ; \Theta ; \Delta \vdash \tau_1 \subty \tau_2 : \star$, and, using $\Theta ; \Delta \vDash \Phi_2 \to \Phi_1$, by S-Impl we have $\Psi ; \Theta ; \Delta \vdash \Phi_1 \implies \tau_1 \subty \Phi_2 \implies \tau_2 : \star$ as required.
  \item[AS-Conj] Suppose $\Psi ; \Theta ; \Delta \vdash \Phi_1 \amp \tau_1 \subtynf \Phi_2 \amp \tau_2 : \star \gens \Phi \wedge (\Phi_1 \to \Phi_2)$ by way of $\Psi ; \Theta ; \Delta \vdash \tau_1 \subtynf \tau_2 : \star \gens \Phi$ with $\Theta ; \Delta \vDash \Phi$ and $\Theta ; \Delta \vDash \Phi_1 \to \Phi_2$. By IH, $\Psi ; \Theta ; \Delta \vdash \tau_1 \subty \tau_2 : \star$, and so by S-Conj, $\Psi ; \Theta ; \Delta \vdash \Phi_1 \amp \tau_1 \subty \Phi_2 \amp \tau_2 : \star$.
  \item[AS-Monad] Suppose $\Psi ; \Theta ; \Delta \vdash M(I,\vec{q}) \tau_1 \subtynf M(J,\vec{p}) \tau_2 : \star \gens (I = J) \wedge (\vec{q} \leq \vec{p}) \wedge \Phi$ by way of $\Psi ; \Theta ; \Delta \vdash \tau_1 \subtynf \tau_2 : \star \gens \Phi$ with $\Theta ; \Delta \vDash (I = J)$,  $\Theta ; \Delta \vDash \vec{q} \leq \vec{p}$, and $\Theta ; \Delta \vDash \Phi$. By IH, $\Psi ; \Theta ; \Delta \vdash \tau_1 \subty \tau_2 : \star$, and since $\Theta ; \Delta \vDash (I = J)$ and $\Theta ; \Delta \vDash \vec{q} \leq \vec{p}$, we have by S-Monad that $\Psi ; \Theta ; \Delta \vdash M(I,\vec{q}) \tau_1 \subty M(J,\vec{p}) \tau_2 : \star$.
  \item[AS-Pot] Suppose $\Psi ; \Theta ; \Delta \vdash [I|\vec{q}] \tau_1 \subtynf [J|\vec{p}] \tau_2 : \star \gens (I = J) \wedge (\vec{p} \leq \vec{q}) \wedge \Phi$ by way of $\Psi ; \Theta ; \Delta \vdash \tau_1 \subtynf \tau_2 : \star \gens \Phi$, with  $\Theta ; \Delta \vDash (I = J)$,  $\Theta ; \Delta \vDash \vec{p} \leq \vec{q}$, and $\Theta ; \Delta \vDash \Phi$. By IH, $\Psi ; \Theta ; \Delta \vdash \tau_1 \subty \tau_2 : \star$. Using the fact that $\Theta ; \Delta \vDash (I = J)$ and $\Theta ; \Delta \vDash \vec{p} \leq \vec{q}$, we have by S-Pot that $\Psi ; \Theta ; \Delta \vdash [i|\vec{q}] \tau_1 \subty [j|\vec{p}] \tau_2 : \star$.
  \item[AS-ConstPot] Suppose ${\Psi ; \Theta ; \Delta \vdash [I] \tau_1 \subtynf [J] \tau_2 : \star \gens \Phi \wedge (J \leq I)}$ by way of ${\Psi ; \Theta ; \Delta \vdash \tau_1 \subtynf \tau_2 : \star \gens \Phi}$ with $\Theta ; \Delta \vDash \Phi$ and $\Theta ; \Delta \vDash J \leq I$. By IH, $\Psi ; \Theta ; \Delta \vdash \tau_1 \subty \tau_2 : \star$, and so using $\Theta ; \Delta \vDash J \leq I$, we have by S-ConstPot that $\Psi ; \Theta ; \Delta \vdash [I] \tau_1 \subty [J] \tau_2 : \star$.
  \item[AS-FamLam] Suppose $\Psi ; \Theta ; \Delta \vdash \lambda i : S. \tau_1 \subtynf \lambda i : S. \tau_2 : S \to K \gens \forall i : S. \Phi$ by way of ${\Psi ; \Theta, i : S ; \Delta \vdash \tau_1 \subtynf \tau_2 : K \gens \Phi}$, with $\Theta ; \Delta \vDash \forall i : S. \Phi$. Equivalently, $\Theta, i : S; \Delta \vDash \Phi$, and so by IH, $\Psi ; \Theta, i : S ; \Delta \vdash \tau_1 \subty \tau_2 : K$, which by S-FamLam means $\Psi ; \Theta ; \Delta \vdash \lambda i : S. \tau_1 \subty \lambda i : S. \tau_2 : S \to K $.
  \item[AS-FamApp] Suppose that $\Psi ; \Theta ; \Delta \vdash \tau_1 \; I \subtynf \tau_2 \; J : K \gens (I = J) \wedge \Phi$ by way of $\Psi ; \Theta ; \Delta \vdash \tau_1 \subtynf \tau_2 : S \to K \gens \Phi$ and $i,j : S  \in \Theta$, with $\Theta ; \Delta \vDash I = J$ and $\Theta ; \Delta \vDash \Phi$. By IH, $\Psi ; \Theta ; \Delta \vdash \tau_1 \subty \tau_2 : S \to K \gens \Phi$, and by S-FamApp, $\Psi ; \Theta ; \Delta \vdash \tau_1 \; I \subty \tau_2 \; J : K$.
\end{itemize}

\end{proof}