\begin{proof}
By induction on $\Psi ; \Theta ; \Delta \vdash \tau_1 \subty \tau_2 : K$.
 \begin{itemize}
   \item[(S-Refl)] Immediate by Theorem~\ref{thm:subty-refl}.
   \item[(S-Trans)] Suppose $\Psi ; \Theta ; \Delta \vdash \tau_1 \subty \tau_3 : K$ by way of $\Psi ; \Theta ; \Delta \vdash \tau_1 \subty \tau_2 : K$ and $\Psi ; \Theta ; \Delta \vdash \tau_2 \subty \tau_3 : K$. By IH, $\Psi ; \Theta ; \Delta \vdash \tau_1 \subty \tau_2 : K \gens \Phi_1$ and $\Psi ; \Theta ; \Delta \vdash \tau_2 \subty \tau_3 : K \gens \Phi_2$ with $\Theta ; \Delta \vDash \Phi_1 \wedge \Phi_2$. But by Theorem~\ref{thm:subty-trans}, we have
   $\Psi ; \Theta ; \Delta \vdash \tau_1 \subty \tau_3 : K \gens \Phi$ and $\Theta ; \Delta \vDash \Phi$, as required.
   \item[(S-Arr)] Suppose $\Psi ; \Theta ; \Delta \vdash \tau_1 \loli \tau_2 \subty \tau_1' \loli \tau_2' : \star$
   from $\Psi ; \Theta ; \Delta \vdash \tau_1' \subty \tau_1 : \star$ and
   $\Psi ; \Theta ; \Delta \vdash \tau_2 \subty \tau_2' : \star$.
   By IH, $\Psi ; \Theta ; \Delta \vdash \tau_1' \subty \tau_1 : \star \gens \Phi_1$,
   and $\Psi ; \Theta ; \Delta \vdash \tau_2 \subty \tau_2' : \star \gens \Phi_2$.
   By inversion, we have $\Psi ; \Theta ; \Delta \vdash \texttt{eval}(\tau_1') \subtynf \texttt{eval}(\tau_1) : \star \gens \Phi_1$
   $\Psi ; \Theta ; \Delta \vdash \texttt{eval}(\tau_2) \subtynf \texttt{eval}(\tau_2') : \star \gens \Phi_2$.
   By AS-Arr,
   $\Psi ; \Theta ; \Delta \vdash \texttt{eval}(\tau_1) \loli \texttt{eval}(\tau_2) \subtynf \texttt{eval}(\tau_1') \loli \texttt{eval}(\tau_2') : \star \gens \Phi_1 \wedge \Phi_2$. But $\texttt{eval}(\tau_1 \loli \tau_2) = \texttt{eval}(\tau_1) \loli \texttt{eval}(\tau_2)$, and so by AS-Normalize, we have
   $\Psi ; \Theta ; \Delta \vdash \tau_1 \loli \tau_2 \subty \tau_1' \loli \tau_2' : \star \gens \Phi_1 \wedge \Phi_2$, as required.
   
   \item[(S-Tensor)] Suppose $\Psi ; \Theta ; \Delta \vdash \tau_1 \otimes \tau_2 \subty \tau_1' \otimes \tau_2' : \star$ from $\Psi ; \Theta ; \Delta \vdash \tau_1 \subty \tau_1' : \star$ and $\Psi ; \Theta ; \Delta \vdash \tau_2 \subty \tau_2' : \star$. By IH, $\Psi ; \Theta ; \Delta \vdash \tau_1 \subty \tau_1' : \star \gens \Phi_1$ and $\Psi ; \Theta ; \Delta \vdash \tau_2 \subty \tau_2' : \star \gens \Phi_2$ with $\Theta ; \Delta \vDash \Phi_1 \wedge \Phi_2$. Inverting both these, we have that $\Psi ; \Theta ; \Delta \vdash \texttt{eval}(\tau_1) \subtynf \texttt{eval}(\tau_1') : \star \gens \Phi_1$ and $\Psi ; \Theta ; \Delta \vdash \texttt{eval}(\tau_2) \subtynf \texttt{eval}(\tau_1') : \star \gens \Phi_2$. By AS-Tensor, $\Psi ; \Theta ; \Delta \vdash \texttt{eval}(\tau_1) \otimes \texttt{eval}(\tau_1') \subtynf \texttt{eval}(\tau_2) \otimes \texttt{eval}(\tau_2') \star \gens \Phi_1 \wedge \Phi_2$. But $\texttt{eval}(\tau \otimes \sigma) = \texttt{eval}(\tau)\otimes\texttt{eval}(\sigma)$ by definition, and so we have by AS-Normalize $\Psi ; \Theta ; \Delta \vdash \tau_1 \otimes \tau_2 \subty \tau_1' \otimes \tau_2' : \star \gens \Phi_1 \wedge \Phi_2$, as required.
   \item[(S-With)] Suppose $\Psi ; \Theta ; \Delta \vdash \tau_1 \amp \tau_2 \subty \tau_1' \amp \tau_2' : \star$ from $\Psi ; \Theta ; \Delta \vdash \tau_1 \subty \tau_1' : \star$ and $\Psi ; \Theta ; \Delta \vdash \tau_2 \subty \tau_2' : \star$. By IH, $\Psi ; \Theta ; \Delta \vdash \tau_1 \subty \tau_1' : \star \gens \Phi_1$ and $\Psi ; \Theta ; \Delta \vdash \tau_2 \subty \tau_2' : \star \gens \Phi_2$ with $\Theta ; \Delta \vDash \Phi_1 \wedge \Phi_2$. Inverting both these, we have that $\Psi ; \Theta ; \Delta \vdash \texttt{eval}(\tau_1) \subtynf \texttt{eval}(\tau_1') : \star \gens \Phi_1$ and $\Psi ; \Theta ; \Delta \vdash \texttt{eval}(\tau_2) \subtynf \texttt{eval}(\tau_1') : \star \gens \Phi_2$. By AS-With, $\Psi ; \Theta ; \Delta \vdash \texttt{eval}(\tau_1) \amp \texttt{eval}(\tau_1') \subtynf \texttt{eval}(\tau_2) \amp \texttt{eval}(\tau_2') \star \gens \Phi_1 \wedge \Phi_2$. But $\texttt{eval}(\tau \amp \sigma) = \texttt{eval}(\tau)\amp\texttt{eval}(\sigma)$ by definition, and so we have by AS-Normalize $\Psi ; \Theta ; \Delta \vdash \tau_1 \amp \tau_2 \subty \tau_1' \amp \tau_2' : \star \gens \Phi_1 \wedge \Phi_2$, as required.
   \item[(S-Sum)] Suppose $\Psi ; \Theta ; \Delta \vdash \tau_1 \oplus \tau_2 \subty \tau_1' \oplus \tau_2' : \star$ from $\Psi ; \Theta ; \Delta \vdash \tau_1 \subty \tau_1' : \star$ and $\Psi ; \Theta ; \Delta \vdash \tau_2 \subty \tau_2' : \star$. By IH, $\Psi ; \Theta ; \Delta \vdash \tau_1 \subty \tau_1' : \star \gens \Phi_1$ and $\Psi ; \Theta ; \Delta \vdash \tau_2 \subty \tau_2' : \star \gens \Phi_2$ with $\Theta ; \Delta \vDash \Phi_1 \wedge \Phi_2$. Inverting both these, we have that $\Psi ; \Theta ; \Delta \vdash \texttt{eval}(\tau_1) \subtynf \texttt{eval}(\tau_1') : \star \gens \Phi_1$ and $\Psi ; \Theta ; \Delta \vdash \texttt{eval}(\tau_2) \subtynf \texttt{eval}(\tau_1') : \star \gens \Phi_2$. By AS-Sum, $\Psi ; \Theta ; \Delta \vdash \texttt{eval}(\tau_1) \oplus \texttt{eval}(\tau_1') \subtynf \texttt{eval}(\tau_2) \oplus \texttt{eval}(\tau_2') \star \gens \Phi_1 \wedge \Phi_2$. But $\texttt{eval}(\tau \oplus \sigma) = \texttt{eval}(\tau)\oplus\texttt{eval}(\sigma)$ by definition, and so we have by AS-Normalize $\Psi ; \Theta ; \Delta \vdash \tau_1 \oplus \tau_2 \subty \tau_1' \oplus \tau_2' : \star \gens \Phi_1 \wedge \Phi_2$, as required.
   \item[(S-Bang)] Suppose $\Psi ; \Theta ; \Delta \vdash !\tau_1 \subty !\tau_2 : \star$ from $\Psi ; \Theta ; \Delta \vdash \tau_1 \subty \tau_2 : \star$.
   By IH, $\Psi ; \Theta ; \Delta \vdash \tau_1 \subty \tau_2 : \star \gens \Phi$ with $\Theta ; \Delta \vDash \Phi$. By inversion, 
   $\Psi ; \Theta ; \Delta \vdash \texttt{eval}(\tau_1) \subtynf \texttt{eval}(\tau_2) : \star \gens \Phi$. By AS-Bang, 
   $\Psi ; \Theta ; \Delta \vdash !\texttt{eval}(\tau_1) \subtynf !\texttt{eval}(\tau_2) : \star \gens \Phi$. But $\texttt{eval}(!\tau) = !\texttt{eval}(\tau)$, and so
    $\Psi ; \Theta ; \Delta \vdash !\tau_1 \subty !\tau_2 : \star \gens \Phi$, as required.
   \item[(S-IForall)] Suppose $\Psi ; \Theta ; \Delta \vdash \forall i : S. \tau_1 \subty \forall i : S. \tau_2 : \star$ from $\Psi ; \Theta, i : S ; \Delta \vdash \tau_1 \subty \tau_2 : \star$. By IH, $\Psi ; \Theta, i : S ; \Delta \vdash \tau_1 \subty \tau_2 : \star \gens \Phi$ with $\Theta, i : S ; \Delta \vDash \Phi$. Equivalently, $\Theta ; \Delta \vDash \forall i : S. \Phi$. By inversion, $\Psi ; \Theta, i : S ; \Delta \vdash \texttt{eval}(\tau_1) \subtynf \texttt{eval}(\tau_2) : \star \gens \Phi$. by AS-IForall, $\Psi ; \Theta ; \Delta \vdash \forall i : S. \texttt{eval}(\tau_1) \subtynf \forall i : S. \texttt{eval}(\tau_2) : \star \gens \forall i : S. \Phi$. But, $\texttt{eval}(\forall i : S. \tau) = \forall i : S.\texttt{eval}(\tau)$, and so by AS-Normalize, $\Psi ; \Theta ; \Delta \vdash \forall i : S. \tau_1 \subty \forall i : S. \tau_2 : \star \gens \forall i : S. \Phi$, as required.
   \item[(S-IExists)] Suppose $\Psi ; \Theta ; \Delta \vdash \exists i : S. \tau_1 \subty \exists i : S. \tau_2 : \star$ from $\Psi ; \Theta, i : S ; \Delta \vdash \tau_1 \subty \tau_2 : \star$. By IH, $\Psi ; \Theta, i : S ; \Delta \vdash \tau_1 \subty \tau_2 : \star \gens \Phi$ with $\Theta, i : S ; \Delta \vDash \Phi$. Equivalently, $\Theta ; \Delta \vDash \forall i : S. \Phi$. By inversion, $\Psi ; \Theta, i : S ; \Delta \vdash \texttt{eval}(\tau_1) \subtynf \texttt{eval}(\tau_2) : \star \gens \Phi$. by AS-IExists, $\Psi ; \Theta ; \Delta \vdash \exists i : S. \texttt{eval}(\tau_1) \subtynf \exists i : S. \texttt{eval}(\tau_2) : \star \gens \forall i : S. \Phi$. But, $\texttt{eval}(\exists i : S. \tau) = \exists i : S.\texttt{eval}(\tau)$, and so by AS-Normalize, $\Psi ; \Theta ; \Delta \vdash \exists i : S. \tau_1 \subty \exists i : S. \tau_2 : \star \gens \forall i : S. \Phi$, as required.
   \item[(S-TForall)] Suppose $\Psi ; \Theta ; \Delta \vdash \forall \alpha : K. \tau_1 \subty \forall \alpha : K. \tau_2 : \star$ from 
   $\Psi, \alpha : K ; \Theta ; \Delta \vdash \tau_1 \subty \tau_2 : \star$. By IH,
   $\Psi, \alpha : K ; \Theta ; \Delta \vdash \tau_1 \subty \tau_2 : \star \gens \Phi$, with $\Theta ; \Delta \vDash \Phi$. By inversion,
   $\Psi, \alpha : K ; \Theta ; \Delta \vdash \texttt{eval}(\tau_1) \subtynf \texttt{eval}(\tau_2) : \star \gens \Phi$. By AS-TForall,
   $\Psi ; \Theta ; \Delta \vdash \forall \alpha : K. \texttt{eval}(\tau_1) \subtynf \forall \alpha : K. \texttt{eval}(\tau_2) : \star \gens \Phi$.
   But, $\texttt{eval}(\forall \alpha : K.\tau) = \forall \alpha : K. \texttt{eval}(\tau)$, and so
   $\Psi ; \Theta ; \Delta \vdash \forall \alpha : K. \tau_1 \subty \forall \alpha : K. \tau_2 : \star \gens \Phi$ by AS-Normalize, as required.
   \item[(S-List)] Suppose $\Psi ; \Theta ; \Delta \vdash L^I \tau_1 \subty L^J \tau_2 : \star$ from
   $\Psi ; \Theta ; \Delta \vdash \tau_1 \subty \tau_2 : \star$ and $\Theta ; \Delta \vDash I = J$.
   By IH, $\Psi ; \Theta ; \Delta \vdash \tau_1 \subty \tau_2 : \star \gens \Phi$ with $\Theta ; \Delta \vDash \Phi$. Consequently, $\Theta l \Delta \vDash \Phi \wedge (I = J)$. By inversion, $\Psi ; \Theta ; \Delta \vdash \texttt{eval}(\tau_1) \subtynf \texttt{eval}(\tau_2) : \star \gens \Phi$. By AS-List,
   $\Psi ; \Theta ; \Delta \vdash L^I\texttt{eval}(\tau_1) \subtynf L^J\texttt{eval}(\tau_2) : \star \gens \Phi \wedge (I = J)$. But, $\texttt{eval}(L^I \tau) = L^I \texttt{eval}(\tau)$, and so by AS-Normalize $\Psi ; \Theta ; \Delta \vdash L^I \tau_1 \subty L^J \tau_2 : \star \gens \Phi \wedge (I = J)$, as required.
   \item[(S-Impl)] Suppose $\Psi ; \Theta ; \Delta \vdash \Phi_1 \implies \tau_1 \subty \Phi_2 \implies \tau_2 : \star$
   from $\Psi ; \Theta ; \Delta \vdash \tau_1 \subty \tau_2 : \star$ and $\Theta;\Delta \vDash \Phi_2 \to \Phi_1$. By IH,
   $\Psi ; \Theta ; \Delta \vdash \tau_1 \subty \tau_2 : \star \gens \Phi$ with $\Theta ; \Delta \vDash \Phi$. Consequently, $\Theta ; \Delta \vDash \phi \wedge (\Phi_2 \to \Phi_1)$. By inversion, $\Psi ; \Theta ; \Delta \vdash \texttt{eval}(\tau_1) \subtynf \texttt{eval}(\tau_2) : \star \gens \Phi$. By AS-Impl,
   $\Psi ; \Theta ; \Delta \vdash \Phi_1 \implies \texttt{eval}(\tau_1) \subtynf \Phi_2 \implies \texttt{eval}(\tau_2) : \star \gens \Phi \wedge (\Phi_2 \to \Phi_1)$. But, $\texttt{eval}(\Phi \implies \tau) = \Phi \implies \texttt{eval}(\tau)$, and so by AS-Normalize,
   $\Psi ; \Theta ; \Delta \vdash \Phi_1 \implies \tau_1 \subty \Phi_2 \implies \tau_2 : \star \gens \Phi \wedge (\Phi_2 \to \Phi_1)$, as required.
   \item[(S-Conj)]  Suppose $\Psi ; \Theta ; \Delta \vdash \Phi_1 \amp \tau_1 \subty \Phi_2 \amp \tau_2 : \star$
   from $\Psi ; \Theta ; \Delta \vdash \tau_1 \subty \tau_2 : \star$ and $\Theta;\Delta \vDash \Phi_1 \to \Phi_2$. By IH,
   $\Psi ; \Theta ; \Delta \vdash \tau_1 \subty \tau_2 : \star \gens \Phi$ with $\Theta ; \Delta \vDash \Phi$. Consequently, $\Theta ; \Delta \vDash \phi \wedge (\Phi_1 \to \Phi_2)$. By inversion, $\Psi ; \Theta ; \Delta \vdash \texttt{eval}(\tau_1) \subtynf \texttt{eval}(\tau_2) : \star \gens \Phi$. By AS-Conj,
   $\Psi ; \Theta ; \Delta \vdash \Phi_1 \amp \texttt{eval}(\tau_1) \subtynf \Phi_2 \amp \texttt{eval}(\tau_2) : \star \gens \Phi \wedge (\Phi_1 \to \Phi_2)$. But, $\texttt{eval}(\Phi \implies \tau) = \Phi \implies \texttt{eval}(\tau)$, and so by AS-Normalize,
   $\Psi ; \Theta ; \Delta \vdash \Phi_1 \amp \tau_1 \subty \Phi_2 \amp \tau_2 : \star \gens \Phi \wedge (\Phi_1 \to \Phi_2)$, as required.
   \item[(S-Monad)] Suppose $\Psi ; \Theta ; \Delta \vdash \M(I,\vec{q}) \tau_1 \subty \M(J,\vec{p}) \tau_2 : \star$ from $\Psi ; \Theta ; \Delta \vdash \tau_1 \subty \tau_2 : \star$ and $\Theta ; \Delta \vDash (I = J) \wedge (\vec{q} \leq \vec{p})$. By IH, $\Psi ; \Theta ; \Delta \vdash \tau_1 \subty \tau_2 : \star \gens \Phi$ with $\Theta ; \Delta \vDash \Phi$. Consequently, $\Theta ; \Delta \vDash \Phi \wedge (I = J) \wedge (\vec{q} \leq \vec{p})$. By inversion,
   $\Psi ; \Theta ; \Delta \vdash \texttt{eval}(\tau_1) \subtynf \texttt{eval}(\tau_2) : \star \gens \Phi$. By AS-Monad,
   $\Psi ; \Theta ; \Delta \vdash \M(I,\vec{q})\texttt{eval}(\tau_1) \subtynf \M(J,\vec{p})\texttt{eval}(\tau_2) : \star \gens \Phi \wedge (I = J) \wedge (\vec{q} \leq \vec{p})$. But, $\texttt{eval}(M(I,\vec{q})\tau)=\M(I,\vec{q})\texttt{eval}(\tau)$, and so by AS-Normalize.
   $\Psi ; \Theta ; \Delta \vdash \M(I,\vec{q}) \tau_1 \subty \M(J,\vec{p}) \tau_2 : \star \gens \Phi \wedge (I = J) \wedge (\vec{q} \leq \vec{p})$, as required.
   \item[(S-Pot)] Suppose $\Psi ; \Theta ; \Delta \vdash [I|\vec{q}] \tau_1 \subty [J|\vec{p}] \tau_2 : \star$ from $\Psi ; \Theta ; \Delta \vdash \tau_1 \subty \tau_2 : \star$ and $\Theta ; \Delta \vDash (I = J) \wedge (\vec{q} \geq \vec{p})$. By IH, $\Psi ; \Theta ; \Delta \vdash \tau_1 \subty \tau_2 : \star \gens \Phi$ with $\Theta ; \Delta \vDash \Phi$. Consequently, $\Theta ; \Delta \vDash \Phi \wedge (I = J) \wedge (\vec{q} \geq \vec{p})$. By inversion,
   $\Psi ; \Theta ; \Delta \vdash \texttt{eval}(\tau_1) \subtynf \texttt{eval}(\tau_2) : \star \gens \Phi$. By AS-Pot,
   $\Psi ; \Theta ; \Delta \vdash [I|\vec{q}]\texttt{eval}(\tau_1) \subtynf [J|\vec{p}]\texttt{eval}(\tau_2) : \star \gens \Phi \wedge (I = J) \wedge (\vec{q} \geq \vec{p})$. But, $\texttt{eval}([I|\vec{q}]\tau)=[I,\vec{q}]\texttt{eval}(\tau)$, and so by AS-Normalize.
   $\Psi ; \Theta ; \Delta \vdash [I|\vec{q}] \tau_1 \subty [J|\vec{p}] \tau_2 : \star \gens \Phi \wedge (I = J) \wedge (\vec{q} \geq \vec{p})$, as required.
   \item[(S-ConstPot)] Suppose $\Psi ; \Theta ; \Delta \vdash [I] \tau_1 \subty [J] \tau_2 : \star$
   from $\Psi ; \Theta ; \Delta \vdash \tau_1 \subty \tau_2 : \star$ and $\Theta;\Delta \vDash J \leq I$.
   By IH, $\Psi ; \Theta ; \Delta \vdash \tau_1 \subty \tau_2 : \star \gens \Phi$ with $\Theta ; \Delta \vDash I \leq J$. Consequently, $\Theta ; \Delta \vDash \Phi \wedge (I \leq J)$. By inversion, $\Psi ; \Theta ; \Delta \vdash \texttt{eval}(\tau_1) \subtynf \texttt{eval}(\tau_2) : \star \gens \Phi$. By AS-ConstPot,
   $\Psi ; \Theta ; \Delta \vdash [I]\texttt{eval}(\tau_1) \subtynf [J]\texttt{eval}(\tau_2) : \star \gens \Phi \wedge (J \leq I)$. But, $\texttt{eval}([I] \tau) = [I]\texttt{eval}(\tau)$, and so by AS-Normalize, $\Psi ; \Theta ; \Delta \vdash [I] \tau_1 \subty [J] \tau_2 : \star \gens \Phi \wedge (J \leq I)$, as required.
   \item[(S-FamLam)] Suppose $\Psi ; \Theta ; \Delta \vdash \lambda i : S. \tau_1 \subty \lambda i : S. \tau_2 : S \to K$
   from $\Psi ; \Theta, i : S ; \Delta \vdash \tau_1 \subty \tau_2 : K$. By IH, $\Psi ; \Theta, i : S ; \Delta \vdash \tau_1 \subty \tau_2 : K \gens \Phi$ with $\Theta, i : S; \Delta \vDash \Phi$, or $\Theta ; \Delta \vDash \forall i : S. \Phi$. By inversion, $\Psi ; \Theta, i : S ; \Delta \vdash \texttt{eval}(\tau_1) \subtynf \texttt{eval}(\tau_2) : K \gens \Phi$. By AS-FamLam, $\Psi ; \Theta ; \Delta \vdash \lambda i : S . \texttt{eval}(\tau_1) \subtynf \lambda i : S.\texttt{eval}(\tau_2) : S \to K \gens \forall i : S. \Phi$. But, $\texttt{eval}(\lambda i : S. \tau) = \lambda i : S. \texttt{eval}(\tau)$, and so by AS-Normalize,
   $\Psi ; \Theta ; \Delta \vdash \lambda i : S. \tau_1 \subty \lambda i : S. \tau_2 : S \to K \gens \forall i : S. \Phi$, as required.
   \item[(S-FamApp)] Suppose $\Psi ; \Theta ; \Delta \vdash \tau_1 \; I \subty \tau_2 \; J : K$ from $\Psi ; \Theta ; \Delta \vdash \tau_1 \subty \tau_2 : S \to K$ and$\Theta ; \Delta \vDash I = J$. By IH,  $\Psi ; \Theta ; \Delta \vdash \tau_1 \subty \tau_2 : S \to K \gens \Phi$ with $\Theta ; \Delta \vDash \Phi$. By inversion, $\Psi ; \Theta ; \Delta \vdash \texttt{eval}(\tau_1) \subtynf \texttt{eval}(\tau_2) : S \to K \gens \Phi$. By Theorem~\ref{thm:eval-app-lemma},
   $\Psi ; \Theta ; \Delta \vdash \texttt{eval}(\tau_1 \; I) \subtynf \texttt{eval}(\tau_2 \; J) : K \gens \Phi'$ with $\Theta ; \Delta \vDash \Phi'$.
   By AS-Normalize, $\Psi ; \Theta ; \Delta \vdash \tau_1 \; I \subty \tau_2 \; J : K \gens \Phi'$, as required.
   
   \item[(S-Fam-Beta1)] Suppose $\Psi ; \Theta ; \Delta \vdash (\lambda i : S. \tau) \; J \subty \tau[J/i] : K$. By AS-Normalize, it suffices to show that
   $\Psi ; \Theta ; \Delta \vdash \texttt{eval}((\lambda i : S. \tau) \; J) \subtynf \texttt{eval}(\tau[J/i]) : K \gens \Phi$ and $\Theta ; \Delta \vDash \Phi$.
   But, $\texttt{eval}((\lambda i : S. \tau) \; J) = \texttt{eval}(\tau)[J/i]$ by definition, and $\texttt{eval}(\tau[J/i]) = \texttt{eval}(\tau)[J/i]$ by Theorem~\ref{thm:idx-subst-eval}. By Theorem~\ref{thm:norm-thm},  $\Psi ; \Theta ; \Delta \vdash \texttt{eval}(\tau)[J/i] : K$, and so by Theorem~\ref{thm:subtynf-refl}, we have that $\Psi ; \Theta ; \Delta \vdash \texttt{eval}(\tau)[J/i] \subtynf \texttt{eval}(\tau)[J/i] : K \gens \Phi$ with $\Theta ; \Delta \vDash \Phi$ as required.
   \item[(S-Fam-Beta2)] Identical to S-FamBeta1.
 \end{itemize}
\end{proof}